work on Infinite Copies

src/tpcms.v
@@ -13,8 +13,10 @@ Require Import Burrow.indexing.
 Require Import Burrow.tactics.
 Require Import coq_tricks.Deex.
 
+Print Is_true.
+
 #[refine]
-Instance pair_tpcm (M: Type) (N: Type)
+Global Instance pair_tpcm (M: Type) (N: Type)
     `{!EqDecision M} `{!TPCM M}
     `{!EqDecision N} `{!TPCM N} : TPCM (M * N) := {
   m_valid p := match p with (m, n) => m_valid m /\ m_valid n end ;
@@ -48,15 +50,17 @@ Class TPCMEmbed (M: Type) (B: Type)
   embed: M -> B ;
   eproject: B -> M ;
   
-  valid_embed: ∀ a , m_valid (embed a) <-> m_valid a ;
-  dot_embed: ∀ a b , dot (embed a) (embed b) = embed (dot a b) ;
-  mov_embed: ∀ a b , mov (embed a) (embed b) <-> mov a b ;
+  valid_embed: ∀ a , m_valid a -> m_valid (embed a) ;
+  valid_eproject: ∀ a , m_valid a -> m_valid (eproject a) ;
+  eproject_dot: ∀ a b , dot (eproject a) (eproject b) = eproject (dot a b) ;
+  mov_embed: ∀ a b , mov a b -> mov (embed a) (embed b) ;
+  mov_eproject: ∀ a b , mov a b -> mov (eproject a) (eproject b) ;
   unit_embed: embed unit = unit ;
   eproject_embed : ∀ a , eproject (embed a) = a ;
 }.
 
 #[refine]
-Instance pair_tpcm_embed_self (M: Type)
+Global Instance pair_tpcm_embed_self (M: Type)
     `{!EqDecision M} `{!TPCM M}
     `{!EqDecision N} `{!TPCM N}
   : TPCMEmbed M M := {
@@ -69,10 +73,12 @@ Proof.
   - intros. trivial.
   - intros. trivial.
   - intros. trivial.
+  - intros. trivial.
+  - intros. trivial.
 Qed.
 
 #[refine]
-Instance pair_tpcm_embed_left (M: Type) (N: Type)
+Global Instance pair_tpcm_embed_left (M: Type) (N: Type)
     `{!EqDecision M} `{!TPCM M}
     `{!EqDecision N} `{!TPCM N}
   : TPCMEmbed M (M * N) := {
@@ -80,20 +86,18 @@ Instance pair_tpcm_embed_left (M: Type) (N: Type)
     eproject := λ p , match p with (m, _) => m end ;
 }.
 Proof.
-  - intros. split.
-    + intro. unfold m_valid in H. unfold pair_tpcm in H. destruct_ands. trivial.
-    + intro. unfold m_valid. unfold pair_tpcm. split; trivial. apply unit_valid.
-  - intros.
-    unfold dot. unfold pair_tpcm. f_equal. apply unit_dot.
-  - intros. split.
-    + intro. unfold mov, pair_tpcm in H. destruct_ands; trivial.
-    + intro. unfold mov, pair_tpcm. split; trivial. apply reflex.
+  - intros. split; trivial. apply unit_valid.
+  - intros. destruct a.
+    unfold m_valid in H. unfold pair_tpcm in H. destruct_ands. trivial.
+  - intros. destruct a, b. unfold dot. unfold pair_tpcm. trivial.
+  - intros. unfold mov, pair_tpcm. split; trivial. apply reflex.
+  - intros. destruct a, b. unfold mov, pair_tpcm in H. destruct_ands; trivial.
   - unfold unit at 3. unfold pair_tpcm. trivial.
   - trivial.
 Defined.
 
 #[refine]
-Instance pair_tpcm_embed_right (M: Type) (N: Type)
+Global Instance pair_tpcm_embed_right (M: Type) (N: Type)
     `{!EqDecision M} `{!TPCM M}
     `{!EqDecision N} `{!TPCM N}
   : TPCMEmbed N (M * N) := {
@@ -101,14 +105,12 @@ Instance pair_tpcm_embed_right (M: Type) (N: Type)
     eproject := λ p , match p with (_, n) => n end ;
 }.
 Proof.
-  - intros. split.
-    + intro. unfold m_valid in H. unfold pair_tpcm in H. destruct_ands. trivial.
-    + intro. unfold m_valid. unfold pair_tpcm. split; trivial. apply unit_valid.
-  - intros.
-    unfold dot. unfold pair_tpcm. f_equal. apply unit_dot.
-  - intros. split.
-    + intro. unfold mov, pair_tpcm in H. destruct_ands; trivial.
-    + intro. unfold mov, pair_tpcm. split; trivial. apply reflex.
+  - intros. split; trivial. apply unit_valid.
+  - intros. destruct a.
+    unfold m_valid in H. unfold pair_tpcm in H. destruct_ands. trivial.
+  - intros. destruct a, b. unfold dot. unfold pair_tpcm. trivial.
+  - intros. unfold mov, pair_tpcm. split; trivial. apply reflex.
+  - intros. destruct a, b. unfold mov, pair_tpcm in H. destruct_ands; trivial.
   - unfold unit at 3. unfold pair_tpcm. trivial.
   - trivial.
 Defined.
@@ -119,22 +121,169 @@ Definition refinement_embed_src R M B
     `{!EqDecision B} `{!TPCM B}
     `{!TPCMEmbed R B} (ref: Refinement R M) : Refinement B M.
 Proof. refine ({|
-  rel_defined := λ b , ∃ r , embed r = b /\ rel_defined R M ref (eproject b) ;
+  rel_defined := λ b , m_valid b /\ rel_defined R M ref (eproject b) ;
   rel := λ b , (rel R M ref (eproject b)) ;
   rel_valid_left := _ ;
   rel_defined_unit := _ ;
   rel_unit := _ ;
   mov_refines := _ ;
 |}).
- - intros. deex. destruct_ands.
-    subst r. rewrite valid_embed.
-      rewrite eproject_embed in H0.
-      apply (rel_valid_left R M ref r0). trivial.
- - exists unit. split.
-    + apply unit_embed.
+ - intros. destruct_ands. trivial.
+ - split.
+    + apply unit_valid.
     + rewrite <- unit_embed. rewrite eproject_embed. apply rel_defined_unit.
  - rewrite <- unit_embed. rewrite eproject_embed. rewrite rel_unit. trivial.
- - intros. deex. destruct_ands. split.
-    + 
+ - intros. destruct_ands. repeat split.
+    + rewrite <- unit_dot in H0.
+      have h := mov_monotonic b b' unit H H0.
+      destruct_ands. rewrite unit_dot in H2. trivial.
+    + assert (mov (eproject b) (eproject b')) as me by (apply mov_eproject; trivial).
+      apply (mov_refines _ _ _ (eproject b)); trivial.
+    + assert (mov (eproject b) (eproject b')) as me by (apply mov_eproject; trivial).
+      apply (mov_refines _ _ _ (eproject b)); trivial.
+Defined.
+
+Definition ic_wf M `{!EqDecision M} `{!TPCM M} (ic_obj: gmap nat M) :=
+  bool_decide (map_Forall (λ _ m, m ≠ unit) ic_obj).
+
+Record InfiniteCopies M `{!EqDecision M} `{!TPCM M} := {
+  ic_obj : gmap nat M ;
+  ic_prf : ic_wf M ic_obj  ;
+}.
+Global Arguments ic_obj {M}%type_scope {EqDecision0 TPCM0} _.
+
+Lemma ic_eq {M} `{!EqDecision M} `{!TPCM M} (ic1 ic2 : InfiniteCopies M)
+    : ic1 = ic2 <-> ic_obj ic1 = ic_obj ic2.
+Proof.
+  split; [by intros ->|intros]. destruct ic1, ic2. simplify_eq/=.
+  f_equal; apply proof_irrel.
+Qed.
+
+Global Instance ic_eq_eq {M} `{!EqDecision M} `{!TPCM M} : EqDecision (InfiniteCopies M). 
+Proof.
+ refine (λ m1 m2, cast_if (decide (ic_obj m1 = ic_obj m2)));
+  abstract (by rewrite ic_eq).
+Defined.
+
+Lemma elem_ne_unit_of_ic_wf {M} `{!EqDecision M} `{!TPCM M} (ic_obj: gmap nat M) i
+  (is_wf: ic_wf M ic_obj)
+  : match ic_obj !! i with
+    | Some x => x ≠ unit
+    | None => True
+  end.
+Proof.
+  unfold ic_wf in is_wf.
+  generalize is_wf.
+  rewrite bool_decide_spec.
+  unfold map_Forall. intros.
+  have h := H i.
+  destruct (ic_obj !! i); trivial.
+  apply h. trivial. Qed.
+
+Definition ic_dot {M} `{!EqDecision M} `{!TPCM M} (a b : InfiniteCopies M) : InfiniteCopies M.
+Proof.
+refine ({|
+  ic_obj := merge (λ x y , match x, y with
+      | None, None => None
+      | Some x, None => Some x
+      | None, Some x => Some x
+      | Some x, Some y => if decide (dot x y = unit) then None else Some (dot x y)
+      end
+  ) (ic_obj a) (ic_obj b) ;
+  ic_prf := _ ;
+|}).
+ - unfold ic_wf.
+    rewrite bool_decide_spec.
+    unfold map_Forall. intros.
+    rewrite lookup_merge in H.
+    destruct a, b.
+    unfold ic_obj in H.
+    unfold diag_None in H. 
     
+    have j1 := elem_ne_unit_of_ic_wf ic_obj0 i ic_prf0.
+    have j2 := elem_ne_unit_of_ic_wf ic_obj1 i ic_prf1.
+    
+    destruct (ic_obj0 !! i), (ic_obj1 !! i); try case_decide; intuition; crush.
+Defined.
+
+Definition ic_get {M} `{!EqDecision M} `{!TPCM M} (a: InfiniteCopies M) (i: nat) : M :=
+  match ic_obj a !! i with
+  | None => unit
+  | Some x => x
+  end.
+
+Definition ic_unit M `{!EqDecision M} `{!TPCM M} : InfiniteCopies M.
+Proof.
+refine ({|
+  ic_obj := empty ;
+  ic_prf := _ ;
+|}).
+ - unfold ic_wf. rewrite bool_decide_spec. unfold map_Forall. intros.
+    rewrite lookup_empty in H. discriminate. Defined.
+
+Definition ic_mov {M} `{!EqDecision M} `{!TPCM M} (a b : InfiniteCopies M) : Prop :=
+  ∀ i , mov (ic_get a i) (ic_get b i).
+
+Lemma ic_get_ic_dot {M} `{!EqDecision M} `{!TPCM M} (x y : InfiniteCopies M) (i : nat)
+  : ic_get (ic_dot x y) i = dot (ic_get x i) (ic_get y i).
+Proof.
+  destruct x, y.
+  unfold ic_get, ic_dot, ic_obj.
+  rewrite lookup_merge.
+  unfold diag_None.
+  destruct (ic_obj0 !! i), (ic_obj1 !! i); try case_decide; intuition; crush.
+  - rewrite unit_dot. trivial.
+  - rewrite unit_dot_left. trivial.
+  - rewrite unit_dot. trivial.
+Qed.
+
+Lemma ic_get_ic_unit {M} `{!EqDecision M} `{!TPCM M} (i : nat)
+  : ic_get (ic_unit M) i = unit.
+Proof.
+  unfold ic_unit, ic_get, ic_obj. rewrite lookup_empty. trivial.
+Qed.
+
+Lemma ic_extens {M} `{!EqDecision M} `{!TPCM M} (a b : InfiniteCopies M)
+  : (∀ i , ic_get a i = ic_get b i) -> a = b.
+Proof.
+  intros. rewrite ic_eq. destruct a, b. unfold ic_obj.
+  apply map_eq. intros. have h := H i. unfold ic_get in h.
+  unfold ic_obj in h.
+  have j1 := elem_ne_unit_of_ic_wf ic_obj0 i ic_prf0.
+  have j2 := elem_ne_unit_of_ic_wf ic_obj1 i ic_prf1.
+  destruct (ic_obj0 !! i), (ic_obj1 !! i); crush.
+Qed.
+
+#[refine]
+Global Instance ic_tpcm (M: Type)
+    `{!EqDecision M} `{!TPCM M} : TPCM (InfiniteCopies M) := {
+  m_valid p := ∀ i , m_valid (ic_get p i) ;
+  dot p1 p2 := ic_dot p1 p2 ;
+  mov p1 p2 := ic_mov p1 p2 ;
+  unit := ic_unit M ;
+}.
+  - intros. have h := H i. rewrite ic_get_ic_dot in h.
+      apply valid_monotonic with (y0 := ic_get y i). trivial.
+  - intros. rewrite ic_get_ic_unit. apply unit_valid.
+  - intros. apply ic_extens. intro. rewrite ic_get_ic_dot.
+      rewrite ic_get_ic_unit. apply unit_dot.
+  - intros. apply ic_extens. intro. repeat (rewrite ic_get_ic_dot).
+      apply tpcm_comm.
+  - intros. apply ic_extens. intro. repeat (rewrite ic_get_ic_dot).
+      apply tpcm_assoc.
+  - intros. unfold ic_mov. intros. apply reflex.
+  - intros. unfold ic_mov in *. intros.
+      have j1 := H i. have j2:= H0 i. apply trans with (y0 := ic_get y i); trivial.
+  - intros. unfold ic_mov in H. split.
+    + intro.
+      have j1 := H i. have j2 := H0 i.
+      rewrite ic_get_ic_dot.
+      rewrite ic_get_ic_dot in j2.
+      apply mov_monotonic with (x0 := ic_get x i); trivial.
+    + unfold ic_mov. intro.
+      have j1 := H i. have j2 := H0 i.
+      rewrite ic_get_ic_dot.
+      rewrite ic_get_ic_dot.
+      rewrite ic_get_ic_dot in j2.
+      apply mov_monotonic with (x0 := ic_get x i); trivial.
 Defined.
